Bwip aux (#14)
* qed on admitted lemmas in BeePL_auxlemmas

* revert changes to fixmes

* merge

* updated access_mode_preserved w/o fixmes

* most of extend_ty_context_deterministic

* some of deref_addr_val_ty

* change extend_ty_context_deterministic to mut ind

* qed on bsem_expr_slv_rlv_ind

* some of expr_spec

* admit old proofs, fix compilation issue in SelectLongproof

* finish mutual induction principles for bsem and ssem

* .

* some proofs in typesystem

* add missing cases to bexpr_cexpr in compiler_proofs

* most of sim_bexpr_cexpr

* qed on preservation lemmas in auxlemmas

* progress in auxlemmas

* fix induction principles in beepl_sem

* fix broken partial proofs in compiler proofs and typesystem

* most of sem_uop_success except for autocasting errors

* fix indP in BeePL_sem

* finish complete me in beepl safety

* some of uop type preserve

* .

* qed on type_translated in compiler_proofs

* match relational spec with compiler in compiler_proofs

* some progress on compiler spec proof

* qed on transBeePL_expr_expr_spec by changing the spec and adding induction princples

* qed on transBeePL_expr_stmt_spec

* fix proof merge issues, make proofs a lot shorter

* remove BeePL_proof.v

* update spec to have bop undef case

* prove transBeePL_function_spec

* prove assign_addr_translated

* prove function return preserved

* fix some proofs with new compiler signature

* fix some proofs in auxlemmas

* some progress towards fixing the spec

* fix EBPF makefile errors

* finish fixing compiler spec, proof is next

* remove old transBeePL_type induction principle

* fix type and expr induction principles

* fix type spec up to type_translated

* complete forgotten merge diff

* update beetypes proofs with map type

* finish updating compiler spec

* change screate to sinit

* some fix with adding maptype

* fix remove maptype and add array

* expr_expr_spec progress

* update

* fix cty_chunk_rel and most of store_well_typed_ext

* some progress

* fix compilation errors

* ref_allocation_succeeds but is actually not possible as stated

* added weaker version of extension but is still not complete, solved deref_addr_value case in store_well_typed_mem_alloc

* Proved store_well_typed_ext_weaker and solved dref_addr_value cases in store_well_typed_alloc

* Almost done with 2nd and third proofs. Need to figure out seperation invariant

* finished proof for storev_succeeds_on_fresh_alloc

* In-progress proofs

* Most lemmas finished, those left need to be resolved with chunk

* Transitionary stage for memory proofs. need to add additional well-formedness definition to make certain proofs correct.

* created new wrappers, and proved/adjusted various lemmas to accomodate for new definition of chunk_of_ptype

* Manual merge and progress on auxillarly lemmas and ebpf properties

* Made it possible to make with code; Next will merge

* fix compilation error

* merged

* edited merge, to make compilation possible

* Finished Lemma 11

* Worked on transBeePL auxillary lemmas; still some of the more complex ones remain to be finished

* cleaned up files

* Removed parameters for well_typed_loc

* some more progress on safe_assgn

* reverted to Swarn's BeePL_auxlemmas.v; fixed troubles for compiling and got as far as possible with memory_proofs.

* some comments in mem_proofs, some fixes in auxlemmas

* Reproduced most of Swarn's proof in ref_allocation_gc; need to figure out same issue (probably requires another assumption) and possible issue in definition of balloc. Fixed more issues in BeePL_auxlemmas.v

* cleaned up some stuff; currently struggling with type mismatch, Value_has_type parallel, and load_not_store

* Adjusted proofs for current changes

* forgot to push BeeTypes

---------

Co-authored-by: Jamie Fulford <47907450+jfulfo@users.noreply.github.com>

beepl/BeeTypes.v
@@ -695,10 +695,10 @@ match t with
 | Tbool => By_value Mbool
 | Tint I8 Signed _ => By_value Mint8signed
 | Tint I8 Unsigned _ => By_value Mint8unsigned
+| Tint IBool _ _ => By_value Mint8unsigned
 | Tint I16 Signed _ => By_value Mint16signed
 | Tint I16 Unsigned _ => By_value Mint16unsigned
 | Tint I32 _ _ => By_value Mint32
-| Tint IBool _ _ => By_value Mint32
 | Tlong _ _ => By_value Mint64
 end.
 
@@ -736,6 +736,7 @@ match ty with
 | Tlong _ _ => BMint64
 end.
 
+(*
 Definition chunk_of_type (ty : type) : option bmemory_chunk :=
 match ty with
 | Vtype pt => Some (chunk_of_ptype pt)
@@ -746,6 +747,18 @@ match ty with
 | Atype _ _ _ => None
 | Ftype _ _ _ _ => None
 | Utype => None
+end.
+*)
+
+Definition chunk_of_type (ty : type) : option bmemory_chunk :=
+match ty with
+| Vtype pt => Some (chunk_of_ptype pt)
+| Utype => None
+| Stype _ _ => None
+| Bytes => None
+| Ftype _ _ _ _ => None
+| Atype _ _ _ => None
+| _ => Some BMint64  (* Assuming 64-bit architecture *)
 end.
 
 Section Eq_basic_types.
