cfrontend/BeePL_auxlemmas.v
@@ -96,60 +96,49 @@ Lemma transBeePL_ptr_ref_bool_int : forall bt a,
 transBeePL_ptr_type (Reftype bt a) = Ctypes.Tpointer (Ctypes.Tint I8 Unsigned noattr) noattr ->
 bt = Bprim Tbool \/ bt = Bprim (Tint I8 Unsigned noattr).
 Proof.
-  (*intros a bt. induction bt; intros; try inv H. generalize dependent a.
-  revert a. induction p; intros; try inv H1. left; auto.
-  right.  auto.
-  induction p; try inv H1.
-Qed.*) Admitted.
+  intros a bt H. induction bt; intros; try inv H. 
+  induction a. induction p. left; auto.
+  right. induction i; induction s; induction a; auto; try inv H1.
+  auto. inv H1. inv H1.
+  right. induction p; auto; try inv H1.
+Qed.
 
 (* Easy *)
 (* Original *)
+(* Don't know if it should be provable *)
 Lemma transBeePL_ptr_ref_bool : forall bt a,
 transBeePL_ptr_type (Reftype bt a) = Ctypes.Tpointer (Ctypes.Tint I8 Unsigned noattr) noattr ->
 bt = Bprim Tbool.
 Proof.
-  (*intros h bt. generalize dependent h. induction bt; intros; try inv H. generalize dependent a.
-  revert h. induction p; intros; try inv H1; auto.
-  - induction h; auto. eapply bprim_bool_int with (h := xH) (bt := Bprim Tbool) (a := noattr). 
-    simpl.  auto.  intro.  inv H. 
-  - destruct p. inv H1. inv H1. inv H1.
-Qed.*) Admitted.
+  intros bt a h.  induction bt; intros; try inv H. generalize dependent a.
+  induction p; intros; try inv H1; auto.
+  - induction i; induction s; induction a; try inv h. auto.
+    admit.
+    inv h. inv h. inv h.
+  - destruct p; try inv H0. 
+Admitted.
 
 Lemma transBeePL_ptr_ref_int_bool : forall bt sz s a a',
 transBeePL_ptr_type (Reftype bt a) = Ctypes.Tpointer (Ctypes.Tint sz s a') a ->
 bt = Bprim (Tint sz s a') \/ bt = Bprim Tbool.
 Proof.
-  (*intro h. induction h; intro bt. induction bt; intros; try inv H. destruct p; try inv H1.
-  destruct IHh with (bt := Bprim Tbool) (sz := I8) (s:= Unsigned) (a':= noattr) (a:= noattr).
-  induction h; auto. left; auto. right; auto. left; auto. destruct p; try inv H1.
-  intros. inv H. destruct bt. destruct p. inv H1.  right; auto.
-  inv H1. left; auto. 
-  inv H1. inv H1. destruct p; try inv H1. 
-  intros. inv H. destruct bt; try inv H1. destruct p; try inv H1; auto. inv H0.
-  left; auto. inv H0. induction p; try inv H0.
-Qed.*) Admitted.
-
+  intro h. induction h; intro bt. induction bt; intros; try inv H. destruct p; try inv H1.
+  right; auto. left; auto.
+  induction p; try inv H1.
+  left; auto. induction p; try inv H1. left; auto.
+  induction p; try inv H1. left; auto.
+  intros. inv H. intros. inv H.
+  induction p; try inv H1.
+Qed.
 
 (* Original *)
 (* Easy *)
+(* Don't think this is possible *)
 Lemma transBeePL_ptr_ref_int : forall bt sz s a a',
 transBeePL_ptr_type (Reftype bt a) = Ctypes.Tpointer (Ctypes.Tint sz s a') a ->
 bt = Bprim (Tint sz s a').
 Proof.
-  (*intro h. induction h; intro bt. induction bt; intros; try inv H. destruct p; try inv H1.
-  destruct IHh with (bt := Bprim Tbool) (sz := I8) (s:= Unsigned) (a':= noattr) (a:= noattr).
-  induction h; auto. auto. auto. destruct p; try inv H1.
-  intros. inv H. destruct bt. destruct p. inv H1. symmetry.
-  apply bprim_bool_int with (h:= xH) (bt := Bprim Tbool) (a := noattr).
-  simpl. auto. intro. inv H.
-  inv H1. auto. inv H1. inv H1. destruct p. inv H1. inv H1. inv H1.
-  intros. inv H. destruct bt. destruct p; try inv H1; auto.
-  symmetry. 
-  apply bprim_bool_int with (h:= xH) (bt := Bprim Tbool) (a := noattr).
-  simpl. auto. intro. inv H.
-  inv H1. destruct p. inv H1. inv H1. inv H1.
-Qed. *) Admitted.
-
+Admitted.
 
 (* Easy *)
 Lemma transBeePL_ptr_ref_long : forall bt s a a',
@@ -213,14 +202,12 @@ Lemma transBeePL_type_pfunction : forall t cts ct c,
 transBeePL_ptr_type t = (Tfunction cts ct c) ->
 exists bts bef brt, t = Fptype bts bef brt (cc_vararg c) /\ transBeePL_types transBeePL_type bts = cts /\ transBeePL_type brt = ct. 
 Proof.
-(*intro.  induction t. induction b. induction p; intros; try inv H.
-intros. inv H. generalize dependent i. revert a0. revert a. revert z.
-induction p; intros; try inv H. intros. inv H. apply IHt in H1.
-destruct H1. destruct H. destruct H. exists x. exists x0.  exists x1.
-split. destruct H. destruct H0. subst. auto. auto. admit.
-split. destruct H. destruct H0. auto.
-destruct H. destruct H0. auto.
-intros. inv H. *)
+intro.  induction t. generalize dependent a. induction b. induction p; intros; try inv H.
+intros. simpl in *. inv H.
+intros. simpl in *. generalize dependent H. revert z a a0 cts ct c. induction p; intros; try inv H.
+intros. simpl in H. inv H.  apply IHt in H1. 
+admit.
+intros. simpl in *. induction l; induction t; auto; try inv H.
 Admitted.
 
 (* Might have to generalize dependent *)
@@ -259,7 +246,9 @@ induction p. simpl in H1.
 induction b; try inv H1. induction p; try inv H0. 
 induction p; try inv H1.
 inv H0. inv H0. inv H0. inv H1. apply IHp in H0. inv H0. 
-inv H1. admit.
+inv H1.
+(* Think this is by design due to definition of transBeePL_type *)
+admit.
 Admitted.
 
 (* Easy *)
@@ -267,19 +256,17 @@ Lemma transBeePL_type_function : forall t cts ct c,
 transBeePL_type t = (Tfunction cts ct c) ->
 exists bts bef brt, t = Ftype bts bef brt (cc_vararg c) /\ transBeePL_types transBeePL_type bts = cts /\ transBeePL_type t = ct. 
 Proof.
-(*induction t; intros; try inv H.
-induction p; try inv H.
-inv H1. inv H1. inv H1.
-induction p; try inv H. simpl in H1.
-induction b; try inv H1. induction p; try inv H1.
-inv H0. inv H0. inv H0. revert H0. generalize dependent i. generalize dependent z.
-generalize dependent a0. generalize dependent a.
-generalize dependent cts. generalize dependent ct. generalize dependent c.
-induction p; intros; try inv H0.
-inv H1. apply IHp in H0. destruct H0. destruct H. destruct H.
-destruct H. destruct H0. exists x. exists x0. exists x1.
-split. subst. symmetry in H. admit.
-inv H. inv H1. admit.*)
+induction t; intros; try inv H.
+induction p; try inv H1.
+induction p; try inv H1. simpl in *.
+induction b; try inv H0. induction p; try inv H1.
+induction p; try inv H1.
+apply IHp in H0. destruct H0 as [bts [bef [brt]]].
+destruct H as [H0 [H1 H2]]. exists bts. exists bef. exists brt.
+split; auto. rewrite <- H0. admit.
+exists l. exists e. exists t.
+split; auto. 
+admit.
 Admitted.
 
 
@@ -346,16 +333,6 @@ Definition access_modeBC (t : type) : mode :=
   | Stype _ _ | Bytes => By_copy
   | _ => access_mode_type t
   end.
-(*
-Definition access_modeBC (t : type) : mode :=
-  match t with
-  | Vtype pt => match pt with
-               | Tbool => By_value Mint8unsigned
-               | pt => access_mode_prim pt
-               end
-  | t => access_mode_type t
-  end.
-*)
 
 Lemma access_mode_preserved : forall ty cty md,
 access_modeBC ty = md ->
@@ -704,47 +681,35 @@ Lemma eq_effect_trans: forall a a0 a1,
     eq_effect_label a a1 ->
     eq_effect_label a0 a1.
 Proof.
-  (*intros. induction a.
+  intros. induction a.
   induction a0; induction a1; auto; try(inv H).
   induction a0; induction a1; auto; try(inv H1).
   induction a0; induction a1; auto; try(inv H).
-  + apply Peqb_true_eq in H2. subst. auto.
-  induction a0; induction a1; auto; try(inv H).
-  +  apply Peqb_true_eq in H2. subst. auto.
-  induction a0; induction a1; auto; try(inv H).
-  +  apply Peqb_true_eq in H2. subst. auto.
-  induction a0; induction a1; auto; try(inv H1).
-Qed.*) Admitted.
+  + destruct a0; destruct a1; try inv a0; try inv a1; auto.
+  + destruct a0; destruct a1; try inv a0; try inv a1; auto.
+  + destruct a0; destruct a1; try inv a0; try inv a1; auto.
+Qed.
   
 Lemma eq_effect_trans': forall a a0 a1,
     eq_effect_label a0 a ->
     eq_effect_label a1 a ->
     eq_effect_label a0 a1.
 Proof.
-  (*intros. induction a.
+  intros. induction a.
   induction a0; induction a1; auto; try(inv H).
   induction a0; induction a1; auto; try(inv H1).
   induction a0; induction a1; auto; try(inv H).
-  + apply Peqb_true_eq in H2. subst. auto.
-    unfold eq_effect_label in *. rewrite Pos.eqb_sym. auto.
-  induction a0; induction a1; auto; try(inv H).
-  + apply Peqb_true_eq in H2. subst. auto.
-    unfold eq_effect_label in *. rewrite Pos.eqb_sym. auto.
-  induction a0; induction a1; auto; try(inv H).
-  + apply Peqb_true_eq in H2. subst. auto.
-    unfold eq_effect_label in *. rewrite Pos.eqb_sym. auto.
-  induction a0; induction a1; auto; try(inv H).
-Qed.*) Admitted.
+  + destruct a0; destruct a1; try inv a0; try inv a1; auto.
+  + destruct a0; destruct a1; try inv a0; try inv a1; auto.
+  + destruct a0; destruct a1; try inv a0; try inv a1; auto.
+Qed.
 
 Lemma eq_effect_sym : forall a b,
     eq_effect_label a b ->
     eq_effect_label b a.
 Proof.
-  (*intros. induction a; induction b; auto.
-  - unfold eq_effect_label in *. rewrite Pos.eqb_sym. auto.
-  - unfold eq_effect_label in *. rewrite Pos.eqb_sym. auto.
-  - unfold eq_effect_label in *. rewrite Pos.eqb_sym. auto.
-Qed.*) Admitted.
+  intros. induction a; induction b; auto.
+Qed.
 
 (* Complete Me: Easy *)
 Lemma sub_effect_trans : forall ef1 ef2 ef3, 
@@ -752,7 +717,7 @@ sub_effect ef1 ef2 = true ->
 sub_effect ef2 ef3 = true ->
 sub_effect ef1 ef3 = true.
 Proof.
-(*  intro. induction ef1.
+intro. induction ef1.
   - intros. apply sub_effect_nil.
   - intros. generalize dependent ef3. induction ef2.
     + intros. inv H.
@@ -781,7 +746,7 @@ Proof.
                      simpl in H0. rewrite Eqa01 in H0.
                      admit.
                      simpl in H0. rewrite Eqa01 in H0. auto.
-                     simpl in Hmid. rewrite Eqaa1 in Hmid. auto.*)
+                     simpl in Hmid. rewrite Eqaa1 in Hmid. auto.
 Admitted.                 
 
 
@@ -1203,4 +1168,3 @@ move=> [].
 + by move=> es e t p /=.
 by move=> p /=.     
 Qed.
-
